EApp works, need to finish admit and other cases

rupicola/io/STLC.fst
@@ -435,7 +435,7 @@ let lem_steps_refl (e:closed_exp) (h:history) : Lemma (steps e e h []) [SMTPat (
   FStar.Squash.return_squash (SRefl e h)
 
 let safe (e:closed_exp) : Type0 =
-  forall (e':closed_exp) (h:history) (lt:local_trace h). steps e e' h lt ==> (is_value e' \/ indexed_can_step e' (h++lt))
+  forall (e':closed_exp) (h:history) (lt:local_trace h). steps e e' h lt ==> (is_value e' \/ can_step e')
 
 let deterministic_path (e':closed_exp) (h:history) (lt:local_trace h) : Type0 =
   forall (e'':closed_exp) (h':history) (lt':local_trace h'). steps e' e'' h' lt' ==> (h' == (h++lt))
@@ -464,40 +464,38 @@ let step_implies_step_for_all_histories (e e':closed_exp) (h:history) (oev:optio
 
 let steps_implies_steps_for_all_histories (e e':closed_exp) (h:history) (lt:local_trace h) :
   Lemma (requires steps e e' h lt)
-        (ensures forall h'. exists lt'. steps e e' h' lt') = admit ()
-
-let can_step_implies_can_step_for_all_histories (e:closed_exp) (h:history) (lt:local_trace h) :
-  Lemma (requires indexed_can_step e (h++lt))
-        (ensures forall h'. exists lt'. indexed_can_step e (h'++lt')) = admit ()
-
+        (ensures forall h'. exists lt'. steps e e' h' lt') =
+  introduce forall h'. exists lt'. steps e e' h' lt' with begin
+    bind_squash #(steps e e' h lt) () (fun sts ->
+    match sts with
+    | SRefl _ _ -> begin
+      assert (steps e e h' [])
+      end
+    | STrans e_step steps_to_e' -> begin
+      admit ()
+      end)
+ end
+     
 let lem_step_preserve_safe (e e':closed_exp) (h:history) (oev:option (event_h h)) :
   Lemma (requires safe e /\ step e e' h oev)
         (ensures safe e') =
-  match oev with
-  | Some ev -> 
-    introduce forall e'' h' lt'. steps e' e'' h' lt' ==> (is_value e'' \/ indexed_can_step e'' (h'++lt')) with begin
-      introduce steps e' e'' h' lt' ==> (is_value e'' \/ indexed_can_step e'' (h'++lt')) with _. begin
-        bind_squash #(steps e' e'' h' lt') () (fun sts ->
-        steps_implies_steps_for_all_histories e' e'' h' lt';
-        assert (forall h_. exists lt_. steps e' e'' h_ lt_);
-        eliminate forall h_. exists lt_. steps e' e'' h_ lt_ with (h++[ev]);
-        assert (exists lt_. steps e' e'' (h++[ev]) lt_);
-        eliminate exists lt_. steps e' e'' (h++[ev]) lt_
-        returns (is_value e'' \/ indexed_can_step e'' (h'++lt')) with _. begin
-          lem_step_implies_steps e e' h oev;
-          assert (steps e e' h [ev]);
-          lem_steps_transitive e e' e'' h [ev] lt_;
-          eliminate forall e' h lt. steps e e' h lt ==> (is_value e' \/ indexed_can_step e' (h++lt)) with e'' h ([ev] @ lt_);
-          assume (is_value e'' \/ indexed_can_step e'' (h'++lt'))
-        end
-        //eliminate forall h_. exists oev_. steps e' e'' h_ oev_ with 
-      //lem_steps_transitive e e' e'' h lt lt';
-      //eliminate forall e' lt. steps e e' h lt ==> (is_value e' \/ indexed_can_step e' (h++lt)) with e'' (lt @ lt');
-      //assert (steps e e'' h (lt @ lt')))
-        )
-      end
+  introduce forall e'' h' lt'. steps e' e'' h' lt' ==> (is_value e'' \/ can_step e'') with begin
+    introduce steps e' e'' h' lt' ==> (is_value e'' \/ can_step e'') with _. begin
+      bind_squash #(steps e' e'' h' lt') () (fun sts ->
+      steps_implies_steps_for_all_histories e' e'' h' lt';
+      assert (forall h_. exists lt_. steps e' e'' h_ lt_);
+      let lt_ev = get_event_trace oev in
+      eliminate forall h_. exists lt_. steps e' e'' h_ lt_ with (h++lt_ev);
+      assert (exists lt_. steps e' e'' (h++lt_ev) lt_);
+      eliminate exists lt_. steps e' e'' (h++lt_ev) lt_
+      returns is_value e'' \/ can_step e'' with _. begin
+        lem_step_implies_steps e e' h oev;
+        assert (steps e e' h lt_ev);
+        lem_steps_transitive e e' e'' h lt_ev lt_;
+        eliminate forall e' h lt. steps e e' h lt ==> (is_value e' \/ can_step e') with e'' h (lt_ev @ lt_)
+      end)
     end
-  | None -> admit ()
+  end
 
 let lem_step_preserve_deterministic_safe (e e':closed_exp) (h:history) (lt:local_trace h) :
   Lemma (requires deterministic_safe e /\ steps e e' h lt)
@@ -531,50 +529,43 @@ let sem_value_shape (t:typ) (e:closed_exp) : Tot Type0 =
   | TArr t1 t2 -> ELam? e
   | TPair t1 t2 -> EPair? e
 
-let sem_expr_shape (t:typ) (e:closed_exp) (h:history) : Tot Type0 =
-  forall (e':closed_exp) (lt:local_trace h). steps e e' h lt ==> irred e' ==> sem_value_shape t e'
+let sem_expr_shape (t:typ) (e:closed_exp) : Tot Type0 =
+  forall (e':closed_exp) (h:history) (lt:local_trace h). steps e e' h lt ==> irred e' ==> sem_value_shape t e'
 
 let deterministic_sem_expr_shape (t:typ) (e:closed_exp) : Type0 =
   forall (e':closed_exp) (h:history) (lt:local_trace h). steps e e' h lt ==> ((irred e' ==> sem_value_shape t e') /\ deterministic_path e' h lt)
 
-let lem_step_preserve_sem_expr_shape (e e':closed_exp) (h:history) (lt:local_trace h) (t:typ) :
+let lem_step_preserve_sem_expr_shape (e e':closed_exp) (h:history) (oev:option (event_h h)) (t:typ) :
   Lemma
-    (requires sem_expr_shape t e h /\ steps e e' h lt)
-    (ensures sem_expr_shape t e' (h++lt)) =
-  introduce forall e'' lt'. steps e' e'' (h++lt) lt' /\ irred e'' ==> sem_value_shape t e'' with begin
+    (requires sem_expr_shape t e /\ step e e' h oev)
+    (ensures sem_expr_shape t e') =
+  introduce forall e'' h' lt'. steps e' e'' h' lt' /\ irred e'' ==> sem_value_shape t e'' with begin
     introduce _  ==> sem_value_shape t e'' with _. begin
-      bind_squash #(steps e' e'' (h++lt) lt') () (fun st ->
-      match st with
-      | SRefl _ _ -> ()
-      | STrans _ _ -> lem_steps_transitive e e' e'' h lt lt')
+      bind_squash #(steps e' e'' h' lt') () (fun st ->
+      steps_implies_steps_for_all_histories e' e'' h' lt';
+      let lt_ev = get_event_trace oev in
+      eliminate forall h_. exists lt_. steps e' e'' h_ lt_ with (h++lt_ev);
+      eliminate exists lt_. steps e' e'' (h++lt_ev) lt_
+      returns sem_value_shape t e'' with _. begin
+        lem_step_implies_steps e e' h oev;
+        lem_steps_transitive e e' e'' h lt_ev lt_;
+        eliminate forall e' h lt. steps e e' h lt /\ irred e' ==> sem_value_shape t e' with e'' h (lt_ev @ lt_)
+      end)
     end
   end
 
-let lem_step_preserve_deterministic_sem_expr_shape (e e':closed_exp) (h:history) (lt:local_trace h) (t:typ) :
-  Lemma
-    (requires deterministic_sem_expr_shape t e /\ steps e e' h lt)
-    (ensures deterministic_sem_expr_shape t e') = admit ()
-  (*introduce forall e'' h' lt'. steps e' e'' h' lt' /\ irred e'' ==> sem_value_shape t e'' with begin
-    introduce _  ==> sem_value_shape t e'' with _. begin
-      bind_squash #(steps e' e'' (h++lt) lt') () (fun st ->
-      match st with
-      | SRefl _ _ -> ()
-      | STrans _ _ -> lem_steps_transitive e e' e'' h lt lt')
-    end
-  end*)
-
 let can_step_eapp_when_safe (e1 e2:closed_exp) (t1 t2:typ) (h:history) : Lemma
   (requires
-    deterministic_safe e1 /\
-    deterministic_safe e2 /\
-    deterministic_sem_expr_shape (TArr t1 t2) e1)
-  (ensures (exists e' oev. step (EApp e1 e2) e' h oev))
-  = admit ()
+    safe e1 /\
+    safe e2 /\
+    sem_expr_shape (TArr t1 t2) e1)
+  (ensures (exists e' h oev. step (EApp e1 e2) e' h oev))
+  =
   (**
      We case analyze if e1 can step or if e2 can step,
        and for each case, we build a step accordingly **)
 
-  (*introduce indexed_irred e1 h /\ indexed_irred e2 h ==> (exists e' oev. step (EApp e1 e2) e' h oev) with _. begin
+  introduce irred e1 /\ irred e2 ==> (exists e' h oev. step (EApp e1 e2) e' h oev) with _. begin
     assert (steps e1 e1 h []);
     assert (steps e2 e2 h []);
     let ELam e11 = e1 in
@@ -582,20 +573,20 @@ let can_step_eapp_when_safe (e1 e2:closed_exp) (t1 t2:typ) (h:history) : Lemma
     ()
   end;
 
-  introduce ~(indexed_irred e1 h) /\ indexed_irred e2 h ==> (exists e' oev. step (EApp e1 e2) e' h oev) with _. begin
+  introduce ~(irred e1) /\ irred e2 ==> (exists e' h oev. step (EApp e1 e2) e' h oev) with _. begin
     assert (steps e2 e2 h []);
-    assert (exists e1' oev1. step e1 e1' h oev1);
-    eliminate exists e1' oev1. step e1 e1' h oev1 returns exists e' oev. step (EApp e1 e2) e' h oev with st. begin
+    assert (exists e1' h oev1. step e1 e1' h oev1);
+    eliminate exists e1' h oev1. step e1 e1' h oev1 returns exists e' h oev. step (EApp e1 e2) e' h oev with st. begin
       bind_squash st (fun st -> return_squash (AppLeft e2 st))
     end
   end;
 
-  introduce ~(irred e2) ==>  (exists e' oev. step (EApp e1 e2) e' h oev) with _. begin
-    assert (exists e2' oev2. step e2 e2' h oev2);
-    eliminate exists e2' oev2. step e2 e2' h oev2 returns exists e' oev. step (EApp e1 e2) e' h oev with st. begin
+  introduce ~(irred e2) ==>  (exists e' h oev. step (EApp e1 e2) e' h oev) with _. begin
+    assert (exists e2' h oev2. step e2 e2' h oev2);
+    eliminate exists e2' h oev2. step e2 e2' h oev2 returns exists e' h oev. step (EApp e1 e2) e' h oev with st. begin
       bind_squash st (fun st -> return_squash (AppRight e1 st))
     end
-  end*)
+  end
 
 (** Such a lemma is mentioned by Amal Ahmed in her PhD thesis, section 2
 
@@ -618,42 +609,6 @@ let can_step_eapp_when_safe (e1 e2:closed_exp) (t1 t2:typ) (h:history) : Lemma
        Subsubcase e2 -> e2'. Similar to above, we use IH.
        Subsubcase irred e2. (From safe e2 we get is_value e2; but not needed by step.)
          So e = EApp (ELam e11) e2 -> subst_beta e2 e11 = e''. Return e11 e2. *)
-
-let transfer_event_between_traces (e e':closed_exp) (h:history) (ev:event_h h) (lt:local_trace (h++[ev])) :
-  Lemma (requires steps e e' (h++[ev]) lt)
-        (ensures steps e e' h ([ev] @ lt)) = admit ()
-
-let no_step_allows_history_extension_safe (e:closed_exp) (h:history) (oev:option (event_h h)):
-  Lemma (requires indexed_safe e h)
-        (ensures indexed_safe e (h++(get_event_trace oev))) =
-  match oev with
-  | Some ev -> begin
-     introduce forall (e':closed_exp) (lt':local_trace (h++[ev])). steps e e' (h++[ev]) lt' ==> (is_value e' \/ indexed_can_step e' ((h++[ev])++lt')) with begin
-       introduce steps e e' (h++[ev]) lt' ==> (is_value e' \/ indexed_can_step e' ((h++[ev])++lt')) with _. begin
-         bind_squash #(steps e e' (h++[ev]) lt') () (fun st ->
-         transfer_event_between_traces e e' h ev lt';
-         eliminate forall e' lt. steps e e' h lt ==> (is_value e' \/ indexed_can_step e' (h++lt)) with e' ([ev] @ lt');
-         ())
-       end
-      end
-    end
-  | None -> ()
-
-let no_step_allows_history_extension_sem_expr_shape (e:closed_exp) (h:history) (oev:option (event_h h)) (t:typ) :
-  Lemma (requires sem_expr_shape t e h)
-        (ensures sem_expr_shape t e (h++(get_event_trace oev))) =
-  match oev with
-  | Some ev -> begin
-     introduce forall (e':closed_exp) (lt':local_trace (h++[ev])). steps e e' (h++[ev]) lt' /\ irred e' ==> sem_value_shape t e' with begin
-       introduce steps e e' (h++[ev]) lt' /\ irred e' ==> sem_value_shape t e' with _. begin
-         bind_squash #(steps e e' (h++[ev]) lt') () (fun st ->
-         transfer_event_between_traces e e' h ev lt';
-         eliminate forall e' lt. steps e e' h lt /\ irred e' ==> sem_value_shape t e' with e' ([ev] @ lt');
-         ())
-       end
-      end
-    end
-  | None -> ()
  
 let rec destruct_steps_eapp
   (e1:closed_exp)
@@ -666,9 +621,9 @@ let rec destruct_steps_eapp
   (t2:typ) :
   Pure (exp * value * (lt2:local_trace h & (lt1:local_trace (h++lt2) & local_trace (((h++lt2)++lt1)))))
     (requires irred e' /\ (** CH: needed, otherwise I can take zero steps; could be replaced by value e' *)
-      deterministic_safe e1 /\
-      deterministic_sem_expr_shape (TArr t1 t2) e1 /\
-      deterministic_safe e2)
+      safe e1 /\
+      sem_expr_shape (TArr t1 t2) e1 /\
+      safe e2)
     (ensures fun (e11, e2', (| lt2, (| lt1, lt3 |) |)) ->
       steps e2 e2' h lt2 /\
       is_closed (ELam e11) /\
@@ -681,9 +636,8 @@ let rec destruct_steps_eapp
     (decreases st)
   = match st with
     | SRefl (EApp e1 e2) h -> begin
-      //can_step_eapp_when_safe e1 e2 t1 t2 h;
-      //false_elim ()
-      admit ()
+      can_step_eapp_when_safe e1 e2 t1 t2 h;
+      false_elim ()
       end
     | STrans #e #f2 #e' #h #_ #lt23 step_eapp step_eapp_steps -> begin
       let (EApp e1 e2) = e in
@@ -693,8 +647,8 @@ let rec destruct_steps_eapp
         lem_step_implies_steps e1 e1' h oev1;
         lem_step_implies_steps (EApp e1 e2) (EApp e1' e2) h oev1;
         let lt1 : local_trace h = get_event_trace oev1 in
-        lem_step_preserve_deterministic_safe e1 e1' h lt1;
-        lem_step_preserve_deterministic_sem_expr_shape e1 e1' h lt1 (TArr t1 t2);
+        lem_step_preserve_safe e1 e1' h oev1;
+        lem_step_preserve_sem_expr_shape e1 e1' h oev1 (TArr t1 t2);
         let s2 : steps (EApp e1' e2) e' (h++lt1) lt23 = step_eapp_steps in
         let (e11, e2', (| _, (| lt1', lt3 |) |)) = destruct_steps_eapp e1' e2 e' (h++lt1) lt23 s2 t1 t2 in
         lem_value_is_irred e2;
@@ -707,7 +661,7 @@ let rec destruct_steps_eapp
         lem_step_implies_steps e2 e2' h oev2;
         lem_step_implies_steps (EApp e1 e2) (EApp e1 e2') h oev2;
         let lt2 : local_trace h = get_event_trace oev2 in
-        lem_step_preserve_deterministic_safe e2 e2' h lt2;
+        lem_step_preserve_safe e2 e2' h oev2;
         let s2 : steps (EApp e1 e2') e' (h++lt2) lt23 = step_eapp_steps in
         let (e11, e2'', (| lt2', (| lt1, lt3 |) |)) = destruct_steps_eapp e1 e2' e' (h++lt2) lt23 s2 t1 t2 in
         lem_steps_transitive e2 e2' e2'' h lt2 lt2';
